Multiple fixes and additions to the CML model

theories/models/utp_cml/utp_cml_commands.thy
@@ -9,7 +9,8 @@ header {* Commands to construct CML definitions *}
 theory utp_cml_commands
 imports 
   utp_cml_functions
-keywords "cmlifun" "cmlefun" :: thy_decl and "inp" "out" "pre" "post"
+  utp_cml_stmt
+keywords "cmlifun" "cmlefun" "cmleop" "cmliop" :: thy_decl and "inp" "out" "pre" "post" "frame"
 begin
 
 abbreviation "swap \<equiv> \<lambda> (x,y). (y, x)"                                          
@@ -21,11 +22,47 @@ definition mk_ifun_body :: "'a set \<Rightarrow> 'b set \<Rightarrow> ('a \<Righ
 declare mk_ifun_body_def [evalp]
 
 ML {*
+
+signature CMLCOMMANDS =
+sig
+  val mk_efun: (string * ((string * string) list * string)) * ((string * string) * string) 
+              -> Proof.context -> local_theory
+  val mk_ifun: (string * ((string * string) list * (string * string))) * (string * string) 
+               -> Proof.context -> local_theory
+  val mk_eop: (string * ((string * string) list * string)) * ((string * string) * string) 
+              -> Proof.context -> local_theory
+  val mk_iop: ((string * ((string * string) list * (string * string))) * (string list * (string * string)))
+              -> Proof.context -> local_theory
+  val efun_pr: Token.T list ->
+      ((string * ((string * string) list * string)) * ((string * string) * string)) * Token.T list
+  val ifun_pr: Token.T list ->
+      ((string * ((string * string) list * (string * string))) * (string * string)) * Token.T list
+  val eop_pr: Token.T list ->
+      ((string * ((string * string) list * string)) * ((string * string) * string)) * Token.T list
+  val iop_pr: Token.T list -> 
+      ((string * ((string * string) list * (string * string))) * (string list * (string * string))) * Token.T list
+end
+
+structure CmlCommands : CMLCOMMANDS =
+struct
+
+open Syntax;
+open Local_Theory;
+
+(* Functions to get grammar categories from the context *)
+
+fun n_upred ctxt = (Config.put root @{nonterminal "n_upred"} ctxt);
+fun n_pexpr ctxt = (Config.put root @{nonterminal "n_pexpr"} ctxt);
+fun vty ctxt = (Config.put root @{nonterminal "vty"} ctxt);
+
+(* Substitute an expression for a given free name irrespective of the type *)
+
 fun subst_free nm e (u $ t) = subst_free nm e u $ subst_free nm e t
   | subst_free nm e (Free (x, t)) = if (x = nm) then e else Free (x, t)
   | subst_free nm e (Abs (y, ty, tr)) = if (nm = y) then (Abs (y, ty, tr)) else (Abs (y, ty, subst_free nm e tr))
   | subst_free _ _ t = t;
 
+(* Insert a lambda abstraction for a given free name, irrespective of the type *)
 local
   fun absnm' x n (u $ t) = (absnm' x n u) $ (absnm' x n t)
     | absnm' x n (Free (y, t)) = if (x = y) then Bound n else Free (y, t)
@@ -33,51 +70,101 @@ local
     | absnm' _ _ e = e;
 in fun absnm (x, ty) n tr = Abs (x, ty, absnm' x n tr) end;
 
-fun get_cml_holty ty ctxt =
-  let val tctxt = (Config.put Syntax.root @{nonterminal "vty"} ctxt) in
-  case (type_of (Syntax.read_term tctxt ty)) of
+(* Given a CML type, get the HOL "maximimal" type *)
+
+fun get_cml_holty ty ctxt = 
+  let val tctxt = vty ctxt in
+  case (type_of (read_term tctxt ty)) of
     Type (_, [ty]) => ty
   | x => error (@{make_string} x)
  end;
 
-local
-  fun mk_lambda' [(id, ty)] n term ctxt =
-        absnm (id, get_cml_holty ty ctxt) n term
-    | mk_lambda' ((id, ty) :: xs) n term ctxt =
-        Const (@{const_name "prod_case"}, dummyT) $ absnm (id, get_cml_holty ty ctxt) n (mk_lambda' xs (n - 1) term ctxt)
-    | mk_lambda' [] _ term _ = term;
-in
-  fun mk_lambda xs term ctxt = mk_lambda' xs (length xs - 1) term ctxt
-end;
+(* Create a product-based lambda term from a list of names and types *)
+
+fun mk_lambda' [(id, ty)] n term ctxt =
+      absnm (id, get_cml_holty ty ctxt) n term
+  | mk_lambda' ((id, ty) :: xs) n term ctxt =
+      const @{const_name "prod_case"} 
+        $ absnm (id, get_cml_holty ty ctxt) n (mk_lambda' xs (n - 1) term ctxt)
+  | mk_lambda' [] _ term _ = term;
+
+fun mk_lambda xs term ctxt = mk_lambda' xs (length xs - 1) term ctxt
+
+(* Attribute to add a theorem to the evalp theorem set *)
 
 val add_evalp = Attrib.internal (K (Thm.declaration_attribute evalp.add_thm));
 
+(* Make a product type from a list of type terms *)
+
+fun mk_prod_ty ctxt [] = @{term UnitD}
+  | mk_prod_ty ctxt ts = foldr1 (fn (x,y) => 
+                           (check_term ctxt (const @{const_abbrev "vty_prod"} $ x $ y)))
+                                            (map (read_term (vty ctxt) o snd) ts)
+
+fun mk_defn id prefix t =
+  ((Binding.name (prefix ^ id), NoSyn), ((Binding.name (prefix ^ id ^ "_def"), [add_evalp]), t))
+
+fun mk_eop ((id, (inp, out)), ((pre, post), body)) ctxt =
+  let val pre_term  = check_term (n_pexpr ctxt) (mk_lambda inp (parse_term (n_pexpr ctxt) pre) ctxt)
+      val post_term = check_term (n_pexpr ctxt)
+                          (const @{const_name "comp"} 
+                            $ (mk_lambda (("RESULT", out) :: inp) (parse_term (n_pexpr ctxt) post) ctxt)
+                            $ const @{const_abbrev "swap"})
+      val body_term = absnm ("RESULT", Type (@{type_abbrev "cmlvar"}, [get_cml_holty out ctxt])) (length inp) (mk_lambda inp (parse_term (n_upred ctxt) body) ctxt)
+      val op_term = check_term ctxt (
+                        const @{const_name CMLOpR} 
+                        $ mk_prod_ty ctxt inp 
+                        $ read_term (vty ctxt) out
+                        $ pre_term
+                        $ post_term
+                        $ body_term)
+      val ((_,(_,thm1)), ctxt1) = define (mk_defn id "pre_" pre_term) ctxt
+      val ((_,(_,thm2)), ctxt2) = define (mk_defn id "post_" post_term) ctxt1
+      val ((_,(_,thm3)), ctxt3) = define (mk_defn id "" op_term) ctxt2
+  in 
+      ctxt3
+  end;
+
+fun mk_iop ((id, (inp, (outn, outt))), (frame, (pre, post))) ctxt =
+let val pre_term  = check_term (n_pexpr ctxt) (mk_lambda inp (parse_term (n_pexpr ctxt) pre) ctxt)
+    val post_term = check_term (n_pexpr ctxt)
+                        (const @{const_name "comp"} 
+                          $ (mk_lambda ((outn, outt) :: inp) (parse_term (n_pexpr ctxt) post) ctxt)
+                          $ const @{const_abbrev "swap"})
+    val frame_set = List.foldr (fn (x, xs) => const @{const_name "finsert"} $ (const @{const_name erase} $ x) $ xs) (const @{const_name "fempty"})
+                               (map (parse_term ctxt) frame)
+    val op_term = check_term ctxt (
+                      const @{const_name CMLIOpR} 
+                      $ mk_prod_ty ctxt inp 
+                      $ read_term (vty ctxt) outt
+                      $ pre_term
+                      $ post_term
+                      $ frame_set)
+      val ((_,(_,thm1)), ctxt1) = define (mk_defn id "pre_" pre_term) ctxt
+      val ((_,(_,thm2)), ctxt2) = define (mk_defn id "post_" post_term) ctxt1
+      val ((_,(_,thm3)), ctxt3) = define (mk_defn id "" op_term) ctxt2
+  in 
+      ctxt3
+  end;
+  
 fun mk_efun ((id, (inp, out)), ((pre, post), body)) ctxt =
-  let val pctxt = (Config.put Syntax.root @{nonterminal "n_pexpr"} ctxt)
-      val tctxt = (Config.put Syntax.root @{nonterminal "vty"} ctxt)
-      val preb = (Binding.name ("pre_" ^ id), NoSyn)
-      val preb_term = Syntax.check_term pctxt (mk_lambda inp (Syntax.parse_term pctxt pre) ctxt)
-      val preb_type = type_of preb_term
-      val preb_def = ( (Binding.name ("pre_" ^ id ^ "_def"), [add_evalp]), preb_term)
-      val bodyb = (Binding.name id, NoSyn)
-      val bodyb_type = Syntax.parse_term tctxt out
-      val bodyb_inner = Syntax.const @{const_name "CoerceD"} 
-                        $ Syntax.parse_term pctxt body (* FIXME: Do something with the postcondition *)
-                        $ bodyb_type
-      val bodyb_def = ( (Binding.name (id ^ "_def"), [add_evalp])
-                      ,  Syntax.check_term pctxt (
-                           mk_lambda inp (
-                             (if (pre = "true") then bodyb_inner
-                                                else Syntax.const @{const_name IfThenElseD}
-                                                   $ Syntax.parse_term pctxt pre
-                                                   $ bodyb_inner 
-                                                   $ Syntax.const @{const_name BotDE})) ctxt))
-      val ((_,(_,thm1)), ctxt1) = Local_Theory.define (preb, preb_def) ctxt
-      val ((_,(_,thm2)), ctxt2) = Local_Theory.define (bodyb, bodyb_def) ctxt1
+  let val pre_term = check_term (n_pexpr ctxt) (mk_lambda inp (parse_term (n_pexpr ctxt) pre) ctxt)
+      val body_type = parse_term (vty ctxt) out
+      val body_inner = const @{const_name "CoerceD"} 
+                       $ parse_term (n_pexpr ctxt) body (* FIXME: Do something with the postcondition *)
+                       $ body_type
+      val body_term = check_term (n_pexpr ctxt) (
+                         mk_lambda inp (
+                           (if (pre = "true") then body_inner
+                                              else const @{const_name IfThenElseD}
+                                                 $ parse_term (n_pexpr ctxt) pre
+                                                 $ body_inner 
+                                                 $ const @{const_name BotDE})) ctxt)
+      val ((_,(_,thm1)), ctxt1) = define (mk_defn id "pre_" pre_term) ctxt
+      val ((_,(_,thm2)), ctxt2) = define (mk_defn id "" body_term) ctxt1
   in 
       ctxt2
   end;
-
 
 fun mk_ifun ((id, (inp, out)), (pre, post)) ctxt = 
   let val pctxt = (Config.put Syntax.root @{nonterminal "n_pexpr"} ctxt)
@@ -92,12 +179,8 @@ fun mk_ifun ((id, (inp, out)), (pre, post)) ctxt =
                             $ (mk_lambda (out :: inp) (Syntax.parse_term pctxt post) ctxt)
                             $ Const (@{const_abbrev "swap"}, dummyT)))
       val postb_def = ( (Binding.name ("post_" ^ id ^ "_def"), [add_evalp]), postb_term) 
-      val inpt = foldr1 (fn (x,y) => 
-            (Syntax.check_term ctxt (Syntax.const @{const_abbrev "vty_prod"} $ x $ y)))
-                                     (map (Syntax.read_term tctxt o snd) inp)
-      val outt = Syntax.read_term tctxt (snd out)
-      val ppctxt = ((Local_Theory.define (preb, preb_def) #> snd) o
-                    (Local_Theory.define (postb, postb_def) #> snd)) ctxt
+      val inpt = mk_prod_ty ctxt inp
+      val outt = read_term tctxt (snd out)
       val bodyb = (Binding.name id, NoSyn)
       val bodyb_def = ( (Binding.name (id ^ "_def"), [add_evalp])
                       ,  Syntax.check_term ctxt (Const (@{const_name mk_ifun_body}, dummyT)
@@ -108,6 +191,8 @@ fun mk_ifun ((id, (inp, out)), (pre, post)) ctxt =
   in 
      ctxt3
   end;
+
+
 
 (*
 fun mk_iop ((id, (inp, out)), (pre, post)) ctxt = 
@@ -141,55 +226,60 @@ fun mk_iop ((id, (inp, out)), (pre, post)) ctxt =
   end;
 *)
 
-val inps_parser = Parse.enum1 "and" (Parse.short_ident -- (@{keyword "::"} |-- Parse.term));
-val outs_parser = Parse.short_ident -- (@{keyword "::"} |-- Parse.term)
+val inps1_pr = Parse.enum1 "and" (Parse.short_ident -- (@{keyword "::"} |-- Parse.term));
+val outs_pr = Parse.short_ident -- (@{keyword "::"} |-- Parse.term)
 
-val cmlifun_parser = Parse.short_ident 
-                  -- ((@{keyword "inp"} |-- inps_parser) -- (@{keyword "out"} |-- outs_parser))
+val ifun_pr = Parse.short_ident 
+                  -- ((@{keyword "inp"} |-- inps1_pr) -- (@{keyword "out"} |-- outs_pr))
                   -- (Scan.optional (@{keyword "pre"} |-- Parse.term) "true"
                       -- (@{keyword "post"} |-- Parse.term));
 
-val cmlefun_parser = Parse.short_ident 
-                  -- ((@{keyword "inp"} |-- inps_parser) -- (@{keyword "out"} |-- Parse.term))
+val efun_pr = Parse.short_ident 
+                  -- ((@{keyword "inp"} |-- inps1_pr) -- (@{keyword "out"} |-- Parse.term))
                   -- ((Scan.optional (@{keyword "pre"} |-- Parse.term) "true"
                   --  (Scan.optional (@{keyword "post"} |-- Parse.term) "true"))
                   --  (@{keyword "is"} |-- Parse.term));
 
+
+
+val eop_pr = Parse.short_ident 
+                  -- ((Scan.optional (@{keyword "inp"} |-- inps1_pr) [("null_input", "()")])
+                      -- (Scan.optional (@{keyword "out"} |-- Parse.term) "()"))
+                  -- ((Scan.optional (@{keyword "pre"} |-- Parse.term) "true"
+                  --  (Scan.optional (@{keyword "post"} |-- Parse.term) "true"))
+                  --  (@{keyword "is"} |-- Parse.term));
+
+val iop_pr = Parse.short_ident 
+                  -- ((Scan.optional (@{keyword "inp"} |-- inps1_pr) [("null_input", "()")])
+                      -- (Scan.optional (@{keyword "out"} |-- outs_pr) ("RESULT", "()")))
+                  -- ((Scan.optional (@{keyword "frame"} |-- Scan.repeat1 Parse.short_ident) []) 
+                  -- (Scan.optional (@{keyword "pre"} |-- Parse.term) "true"
+                      -- (@{keyword "post"} |-- Parse.term)));
+
+end;
+
+
+
+
+Scan.optional;
+
 Outer_Syntax.local_theory  @{command_spec "cmlefun"} 
 "Explicit CML function" 
-(cmlefun_parser >> mk_efun);
+(CmlCommands.efun_pr >> CmlCommands.mk_efun);
 
 Outer_Syntax.local_theory  @{command_spec "cmlifun"} 
 "Implicit CML function" 
-(cmlifun_parser >> mk_ifun);
+(CmlCommands.ifun_pr >> CmlCommands.mk_ifun);
+
+Outer_Syntax.local_theory  @{command_spec "cmliop"} 
+"Implicit CML operation" 
+(CmlCommands.iop_pr >> CmlCommands.mk_iop);
+
+Outer_Syntax.local_theory  @{command_spec "cmleop"} 
+"Explicit CML operation" 
+(CmlCommands.eop_pr >> CmlCommands.mk_eop);
 
 *}
-
-ML {*  *}
-
-ML {* Attrib.internal (K Simplifier.simp_add) *}
-
-
-cmlifun mydiv
-  inp x :: "@nat" and y :: "@nat"
-  out z :: "@nat"
-  pre "&y > 0" 
-  post "&z = floor (&x / &y)"
-
-thm evalp
-
-print_theorems
-
-cmlefun myadd
-  inp x :: "@nat" and y :: "@nat"
-  out "@real"
-  pre "&x > 0"
-  is "&x + &y"
-
-thm evalp
-
-lemma "((4,2),2) \<in> mydiv"
-  by (simp add:evalp)
 
 end
 
